Proof of eutt -> trace_eq

theories/Trace.v
@@ -2,34 +2,207 @@ Require Import List.
 Import ListNotations.
 
 From ITree Require Import
-     Core.
+     Core
+     Eq.Eq
+     Eq.UpToTaus.
+
+From Paco Require Import
+     paco.
 
 Inductive event (E : Type -> Type) : Type :=
-| Event : forall X, E X -> X -> event E.
+| Event : forall X, E X -> X -> event E
+| OutputEvent : forall X, E X -> event E
+.
 
 Arguments Event {E X}.
+Arguments OutputEvent {E X}.
 
 Definition trace (E : Type -> Type) : Type := list (event E).
 
-Inductive is_trace {E : Type -> Type} {R : Type} :
-  itree E R -> trace E -> option R -> Prop :=
-| TraceEmpty : forall t, is_trace t [] None
-| TraceRet : forall r, is_trace (Ret r) [] (Some r)
+Inductive is_traceF {E : Type -> Type} {R : Type} :
+  itreeF E R (itree E R) -> trace E -> option R -> Prop :=
+| TraceEmpty : forall t, is_traceF t [] None
+| TraceRet : forall r,
+    is_traceF (RetF r) [] (Some r)
 | TraceTau : forall t tr r_,
-  is_trace t tr r_ ->
-  is_trace (Tau t) tr r_
+    is_traceF (observe t) tr r_ ->
+    is_traceF (TauF t) tr r_
 | TraceVis : forall X (e : E X) (x : X) k tr r_,
-  is_trace (k x) tr r_ ->
-  is_trace (Vis e k) (Event e x :: tr) r_
+    is_traceF (observe (k x)) tr r_ ->
+    is_traceF (VisF e k) (Event e x :: tr) r_
+| TraceUninhab : forall X (e : E X) k,
+    is_traceF (VisF e k) [OutputEvent e] None
 .
 
+Definition is_trace {E R} (t : itree E R) := is_traceF (observe t).
+
+(* t1 ⊑ t2 *)
 Definition trace_incl {E : Type -> Type} {R : Type} :
   itree E R -> itree E R -> Prop :=
   fun t1 t2 =>
     forall tr r_, is_trace t1 tr r_ -> is_trace t2 tr r_.
 
+(* t1 ≡ t2 *)
+Definition trace_eq {E R} : itree E R -> itree E R -> Prop :=
+  fun t1 t2 =>
+    trace_incl t1 t2 /\ trace_incl t2 t1.
+
+Require Import ProofIrrelevance.
+
+Ltac invert_existTs :=
+  repeat match goal with
+         | [ H : existT ?P ?p _ = existT ?P ?p _ |- _ ] => apply inj_pair2 in H
+         end; subst.
+
+(* A trace is still valid after removing taus *)
+Lemma is_trace_unalltaus: forall {E R} (t1 t2 : itree E R) tr r,
+    unalltausF (observe t1) (observe t2) ->
+    is_trace t1 tr r ->
+    is_trace t2 tr r.
+Proof.
+  intros. induction H0; intros; subst; try solve [constructor].
+  - inv H; subst. inv H0; subst.
+    + red. rewrite <- H3. constructor.
+    + inversion OBS.
+  - apply IHis_traceF. eapply unalltaus_tau; eauto.
+  - red. destruct (observe t2).
+    + inv H. inv H1. inv OBS.
+    + inv H. inv H2.
+    + inv H. inv H1.
+      * invert_existTs. constructor; auto.
+      * inv OBS.
+  - red. destruct (observe t2).
+    + inv H. inv H0. inv OBS.
+    + inv H. inv H1.
+    + inv H. inv H0.
+      * invert_existTs. constructor.
+      * inv OBS.
+Qed.
+
+(* A trace is still valid after adding taus *)
+Lemma is_trace_unalltaus': forall {E R} (t1 t2 : itree E R) tr r,
+    unalltausF (observe t1) (observe t2) ->
+    is_trace t2 tr r ->
+    is_trace t1 tr r.
+Proof.
+  intros. inversion H. remember (observe t1). remember (observe t2).
+  generalize dependent t1. generalize dependent t2. induction H1; intros; subst.
+  - red. rewrite <- Heqi. assumption.
+  - red. rewrite <- Heqi. constructor. eapply IHuntausF; auto.
+Qed.
+
+Lemma euttF_tau_add {E R} r (t1 t2 t1' : itree E R)
+    (OBS: TauF t1' = observe t1)
+    (REL: eutt_ r t1' t2):
+  eutt_ r t1 t2.
+Proof.
+  intros. destruct REL. econstructor.
+  - rewrite finite_taus_tau; eauto.
+  - intros. eapply EQV; eapply unalltaus_tau; eauto.
+    inversion UNTAUS2. constructor; auto. econstructor; eauto.
+Qed.
+
+Lemma euttF_tau_remove {E R} r (t1 t2 t1' : itree E R)
+    (OBS: TauF t1 = observe t1')
+    (REL: eutt_ r t1' t2):
+  eutt_ r t1 t2.
+Proof.
+  intros. destruct REL. econstructor.
+  - rewrite <- FIN. symmetry. rewrite finite_taus_tau; eauto. reflexivity.
+  - intros. eapply EQV; eauto. rewrite <- OBS. inversion UNTAUS1. constructor; auto.
+    econstructor; eauto.
+Qed.
+
+Lemma euttF_tau_remove' {E R} r (t1 t2 t2' : itree E R)
+    (OBS: TauF t2 = observe t2')
+    (REL: eutt_ r t1 t2'):
+  eutt_ r t1 t2.
+Proof.
+  intros. destruct REL. econstructor.
+  - rewrite FIN. rewrite finite_taus_tau; eauto. reflexivity.
+  - intros. eapply EQV; eauto. rewrite <- OBS. inversion UNTAUS2. constructor; auto.
+    econstructor; eauto.
+Qed.
+
+Lemma eutt_trace_incl : forall {E R} (t1 t2 : itree E R),
+    t1 ~~ t2 -> trace_incl t1 t2.
+Proof.
+  red. intros. red in H0. remember (observe t1).
+  generalize dependent t1. generalize dependent t2.
+  induction H0; intros; try solve [constructor].
+  - pinversion H.
+    assert (Hunall: unalltausF (observe t1) (RetF r)).
+    {
+      rewrite Heqi. constructor; auto. red. rewrite <- Heqi. auto.
+    }
+    assert (FIN2: finite_tausF (observe t1)) by (eexists; apply Hunall).
+    rewrite FIN in FIN2. inv FIN2.
+    specialize (EQV _ _ Hunall H0). inv EQV. red.
+    eapply is_trace_unalltaus'.
+    + simpobs. auto.
+    + red. rewrite <- Heqi. constructor.
+  - apply IHis_traceF with (t1:=t); auto.
+    rewrite <- H. symmetry. apply tauF_eutt. assumption.
+  - pinversion H.
+    assert (Hunall: unalltausF (observe t1) (VisF e k)).
+    {
+      rewrite Heqi. constructor; auto. red. rewrite <- Heqi. auto.
+    }
+    assert (FIN2: finite_tausF (observe t1)) by (eexists; apply Hunall).
+    rewrite FIN in FIN2. inv FIN2.
+    specialize (EQV _ _ Hunall H1). inv EQV.
+    invert_existTs. inv H1. specialize (H6 x).
+
+    red. remember (VisF _ _) in H2. remember (observe t2).
+    generalize dependent t2.
+    induction H2; intros; subst.
+    + constructor. apply IHis_traceF with (t1:=k x); auto.
+      pfold. inversion H6.
+      pinversion H1. inversion H1.
+    + constructor. eapply IHuntausF; auto.
+      * rewrite FIN. apply finite_taus_tau; auto.
+      * eapply euttF_tau_remove'; eauto.
+  - pinversion H.
+    assert (Hunall: unalltausF (observe t1) (VisF e k)).
+    {
+      rewrite Heqi. constructor; auto. red. rewrite <- Heqi. auto.
+    }
+    assert (FIN2: finite_tausF (observe t1)) by (eexists; apply Hunall).
+    rewrite FIN in FIN2. inv FIN2.
+    specialize (EQV _ _ Hunall H0). inv EQV.
+    invert_existTs. inv H0.
+
+    red. remember (VisF _ _) in H1. remember (observe t2).
+    generalize dependent t2.
+    induction H1; intros; subst; constructor.
+    eapply IHuntausF; auto.
+    + rewrite FIN. apply finite_taus_tau; auto.
+    + eapply euttF_tau_remove'; eauto.
+Qed.
+
+Lemma eutt_trace_eq : forall {E R} (t1 t2 : itree E R),
+    t1 ~~ t2 -> trace_eq t1 t2.
+Proof.
+  split.
+  - apply eutt_trace_incl; auto.
+  - symmetry in H. apply eutt_trace_incl; auto.
+Qed.
+
+Lemma trace_eq_eutt : forall {E R} (t1 t2 : itree E R),
+    trace_eq t1 t2 -> t1 ~~ t2.
+Proof.
+Admitted.
+
+Theorem trace_eq_iff_eutt : forall {E R} (t1 t2 : itree E R),
+    t1 ~~ t2 <-> trace_eq t1 t2.
+Proof.
+  split.
+  - apply eutt_trace_eq.
+  - apply trace_eq_eutt.
+Qed.
+
 (* [step_ ev t' t] if [t] steps to [t'] (read right to left!)
-   with visible event [ev]. *) 
+   with visible event [ev]. *)
 Inductive step_ {E : Type -> Type} {R : Type}
           (ev : event E) (t' : itree E R) :
   itree E R -> Prop :=
